theories/logrel/ftlr_yield.v
@@ -52,7 +52,7 @@ Lemma ftlr_yield {i mem_acc_tx ai regs rxs ps_acc p_tx p_rx instr trans r0}:
               (∃ mem : lang.mem, memory_pages (a0 ∪ (accessible_in_trans_memory_pages i a1)) mem) -∗
               ((∃ r0 : Addr, R0 @@ V0 ->r r0 ∗ ⌜decode_hvc_func r0 = Some Run⌝) ∗
               (∃ r1 : Addr, R1 @@ V0 ->r r1 ∗ ⌜decode_vmid r1 = Some i⌝) ∗ (∃ r2 : Addr, R2 @@ V0 ->r r2) ∗
-              ▷ VMProp V0 (vmprop_zero i a1 a2) (1 / 2) ∗ VMProp i (vmprop_unknown i) 1) -∗
+              ▷ VMProp V0 (vmprop_zero i a1 a2) (1 / 2) ∗ ∃ P, VMProp i P 1) -∗
               WP ExecI @ i {{ _, True }}) -∗
    ([∗ map] r↦w ∈ regs, r @@ i ->r w) -∗
    TX@i:=p_tx -∗
@@ -72,7 +72,7 @@ Lemma ftlr_yield {i mem_acc_tx ai regs rxs ps_acc p_tx p_rx instr trans r0}:
    (∃ mem2 : mem, memory_page p_tx mem2) -∗
    ((∃ r0 : Addr, R0 @@ V0 ->r r0 ∗ ⌜decode_hvc_func r0 = Some Run⌝) ∗
     (∃ r1 : Addr, R1 @@ V0 ->r r1 ∗ ⌜decode_vmid r1 = Some i⌝) ∗ (∃ r2 : Addr, R2 @@ V0 ->r r2) ∗
-    ▷ VMProp V0 (vmprop_zero i trans rxs) (1 / 2) ∗ VMProp i (vmprop_unknown i) 1) -∗
+    ▷ VMProp V0 (vmprop_zero i trans rxs) (1 / 2) ∗ ∃ P, VMProp i P 1) -∗
    SSWP ExecI @ i {{ bm, (if bm.1 then VMProp_holds i (1 / 2) else True) -∗ WP bm.2 @ i {{ _, True }} }}.
   Proof.
     iIntros (Htotal_regs Htotal_rxs Hsubset_mb Hneq_0 Hsubset_acc Hnin_rx Hnin_tx Hlookup_PC Hin_ps_acc Hneq_ptx Hdom_mem_acc_tx Hin_ps_acc_tx
@@ -159,6 +159,7 @@ Lemma ftlr_yield {i mem_acc_tx ai regs rxs ps_acc p_tx p_rx instr trans r0}:
       iDestruct (mem_big_sepM_split mem_oea Hlookup_mem_ai' with "mem_oea") as "[mem_instr Hacc_mem]".
       iDestruct ("tx") as "#tx".
       iAssert (RX@i := p_rx)%I  with "[rx]" as "#rx'". iDestruct "rx" as "[$ ?]".
+      iDestruct "propi" as "[% propi]".
       iApply (yield ai (transaction_hpool_global_transferred trans ∗
                         transaction_pagetable_entries_transferred i trans ∗
                         retrievable_transaction_transferred i trans)%I _
@@ -184,6 +185,7 @@ Lemma ftlr_yield {i mem_acc_tx ai regs rxs ps_acc p_tx p_rx instr trans r0}:
         iFrame "mem_trans".
         rewrite memory_pages_singleton'.
         iSplit. iPureIntro. apply only_except_disjoint.
+        iSplit. iPureIntro. split;done.
         iSplitL "mem_rx". iExists p_rx. iFrame "rx' mem_rx".
         iSplitR "propi".
         iLeft. iFrame. iExists _. iFrame "R2z".
@@ -199,9 +201,8 @@ Lemma ftlr_yield {i mem_acc_tx ai regs rxs ps_acc p_tx p_rx instr trans r0}:
       iEval (rewrite later_exist) in "Hres". iDestruct "Hres" as (trans') "Hres".
       iEval (rewrite later_exist) in "Hres". iDestruct "Hres" as (rxs') "Hres".
       iEval (rewrite 11!later_sep) in "Hres".
-      iDestruct "Hres" as "(>trans_hpool_global & >tran_pgt_transferred &
+      iDestruct "Hres" as "(>%trans_rel & >trans_hpool_global & >tran_pgt_transferred &
                          >retri & >mem_transferred & >R0z & >R1z & >R2z & (>rx_state & >[% [rx'' [% mem_rx]]]) & >other_rx & >%Htotal_rxs' & prop0)".
-      iDestruct (get_trans_rel_secondary with "[$trans_hpool_global $retri $tran_pgt_owned $retri_owned]") as "%trans_rel".
       erewrite (trans_rel_secondary_currently_accessible_memory_pages);eauto.
       erewrite (trans_rel_secondary_currently_accessible_memory_pages) in Hsubset_acc;eauto.
       iDestruct (trans_rel_secondary_transaction_pagetable_entries_owned with "tran_pgt_owned") as "tran_pgt_owned";eauto.
@@ -268,7 +269,8 @@ Lemma ftlr_yield {i mem_acc_tx ai regs rxs ps_acc p_tx p_rx instr trans r0}:
       }
       iApply ("IH" $! _ ps_acc trans' _ Htotal_rxs' Htotal_regs' Hsubset_mb Hsubset_acc Hnin_rx' Hnin_tx' with "regs'' tx pgt_tx rx pgt_acc pgt_owned
                        trans_hpool_global tran_pgt_transferred retri  rx_state other_rx
-                           tran_pgt_owned retri_owned mem [$R0z $R1z $R2z $prop0 $propi]").
+                           tran_pgt_owned retri_owned mem [$R0z $R1z $R2z $prop0 propi]").
+      iExists _. done.
     }
     { (* tpa ai ∉ ps_acc ∖ ({[p_rx]} ∪ ps_mem_in_trans) *)
       (* we don't need to touch [mem_oea]*)
@@ -295,6 +297,7 @@ Lemma ftlr_yield {i mem_acc_tx ai regs rxs ps_acc p_tx p_rx instr trans r0}:
       iDestruct (mem_big_sepM_split mem_inters Hlookup_mem_ai' with "mem_inters") as "[mem_instr Hacc_mem_inters]".
       iDestruct ("tx") as "#tx".
       iAssert (RX@i := p_rx)%I  with "[rx]" as "#rx'". iDestruct "rx" as "[$ ?]".
+      iDestruct "propi" as "[% propi]".
       iApply (yield ai (transaction_hpool_global_transferred trans ∗
                         transaction_pagetable_entries_transferred i trans ∗
                         retrievable_transaction_transferred i trans) _
@@ -332,6 +335,7 @@ Lemma ftlr_yield {i mem_acc_tx ai regs rxs ps_acc p_tx p_rx instr trans r0}:
         iFrame "mem_trans".
         rewrite memory_pages_singleton'.
         iSplit. iPureIntro. apply only_except_disjoint.
+        iSplit. iPureIntro. split;done.
         iSplitL "mem_rx". iExists p_rx. iFrame "rx' mem_rx".
         iSplitR "propi".
         iLeft. iFrame. iExists _. iFrame.
@@ -345,10 +349,9 @@ Lemma ftlr_yield {i mem_acc_tx ai regs rxs ps_acc p_tx p_rx instr trans r0}:
       iEval (rewrite later_exist) in "Hres". iDestruct "Hres" as (trans') "Hres".
       iEval (rewrite later_exist) in "Hres". iDestruct "Hres" as (rx_state') "Hres".
       iEval (rewrite 11!later_sep) in "Hres".
-      iDestruct "Hres" as "(>trans_hpool_global & >tran_pgt_transferred &
+      iDestruct "Hres" as "(>%trans_rel & >trans_hpool_global & >tran_pgt_transferred &
                          >retri & >mem_transferred & >R0z & >R1z & >R2z & (>rx_state & >[% [rx'' [% mem_rx]]]) & >other_rx & >%Htotal_rxs' & prop0)".
       iDestruct ("Hacc_regs" $! (ai ^+ 1)%f r0 with "[PC R0i]") as "[%regs' [%Htotal_regs' regs'']]"; iFrameAutoSolve.
-      iDestruct (get_trans_rel_secondary with "[$trans_hpool_global $retri $tran_pgt_owned $retri_owned]") as "%trans_rel".
       erewrite (trans_rel_secondary_currently_accessible_memory_pages);eauto.
       erewrite (trans_rel_secondary_currently_accessible_memory_pages) in Hsubset_acc;eauto.
       iDestruct (trans_rel_secondary_transaction_pagetable_entries_owned with "tran_pgt_owned") as "tran_pgt_owned";eauto.
@@ -414,7 +417,8 @@ Lemma ftlr_yield {i mem_acc_tx ai regs rxs ps_acc p_tx p_rx instr trans r0}:
       }
       iApply ("IH" $! _ ps_acc trans' _ Htotal_rxs' Htotal_regs' Hsubset_mb Hsubset_acc Hnin_rx' Hnin_tx' with "regs'' tx pgt_tx rx pgt_acc pgt_owned
                        trans_hpool_global tran_pgt_transferred retri rx_state other_rx
-                           tran_pgt_owned retri_owned mem [$R0z $R1z $R2z $prop0 $propi]").
+                           tran_pgt_owned retri_owned mem [$R0z $R1z $R2z $prop0 propi]").
+      iExists _. done.
     }
   Qed.
 
